Decode request and response

theories/Decode.v
@@ -17,17 +17,14 @@ Definition dparse {T} (pr : parser T) (s : string) : string + T :=
 Definition dpath' {T} (d : JDecode T) (s : string) (j : json) : string + T :=
   decode__jpath (s -> this) j >>= d.
 
-Definition dpath {T} `{JDecode T} : string -> json -> string + T :=
-  dpath' decode.
+Definition dpath {T} `{JDecode T} : string -> JDecode T := dpath' decode.
 
 Instance JDecode__Method : JDecode request_method :=
   fun j => dpath "method" j >>= dparse parseMethod.
 
-Definition decode__path : JDecode path :=
-  fun j => dpath "path" j.
+Definition decode__path : JDecode path := dpath "path".
 
-Definition decode__oquery : JDecode (option query) :=
-  fun j => dpath "query" j.
+Definition decode__oquery : JDecode (option query) := dpath "query".
 
 Definition decode__origin : JDecode request_target :=
   fun j => liftA2 RequestTarget__Origin (decode__path j) (decode__oquery j).
@@ -49,9 +46,32 @@ Instance JDecode__RequestTarget : JDecode request_target :=
         RequestTarget__Authority <$> dpath "authority" j <|>
         inr RequestTarget__Asterisk.
 
-Instance JDecode__Version : JDecode http_version :=
+Definition decode__version : JDecode http_version :=
   fun j => liftA2 Version (dpath "major" j) (dpath "minor" j).
 
+Instance JDecode__version : JDecode http_version :=
+  fun j => (dpath' decode__version "version" j) <|> inr (Version 1 1).
+
 Instance JDecode__RequestLine : JDecode request_line :=
-  fun j => liftA2 RequestLine (decode j) (dpath "target" j) <*>
-               (dpath "version" j).
+  fun j => liftA2 RequestLine (decode j) (dpath "target" j) <*> (decode j).
+
+Instance JDecode__Field : JDecode (field_line id) :=
+  fun j => liftA2 Field (dpath "name" j) (dpath "value" j).
+
+Instance JDecode__Request : JDecode (http_request id) :=
+  fun j => liftA2 Request (decode j) (dpath "fields" j) <*> (dpath "body" j).
+
+Instance JDecode__Status : JDecode status_line :=
+  fun j => liftA2 Status (decode j) (dpath "code" j) <*> (dpath "phrase" j).
+
+Instance JDecode__Response : JDecode (http_response id) :=
+  fun j => liftA2 Response (decode j) (dpath "fields" j) <*> (dpath "body" j).
+
+Definition request_of_json (j : json) : http_request id :=
+  if decode j is inr req then req
+  else Request (RequestLine (Method "BREW") RequestTarget__Asterisk (Version 1 0))
+               [] None.
+
+Definition response_of_json (j : json) : http_response id :=
+  if decode j is inr res then res
+  else Response (Status (Version 1 0) 418 None) [] None.
